#+TITLE: Maths Notes

* Trigonometry
** Reciprocal Trigonometric Functions

The identity $\sin^{2}(\theta) + \cos^{2}(\theta) = 1$ is the foundation for two more complex identities.

Dividing by $\cos^{2}(\theta)$:

- \[\dfrac{\sin^{2}(\theta)}{\cos^{2}(\theta)}+ \dfrac{\cos^{2}(\theta)}{\cos^{2}(\theta)} = \dfrac{1}{cos^{2}(\theta)}\]

Dividing by $\sin^{2}(\theta)$:

- \[\dfrac{\sin^{2}(\theta)}{\sin^{2}(\theta)}+ \dfrac{\cos^{2}(\theta)}{\sin^{2}(\theta)} = \dfrac{1}{sin^{2}(\theta)}\]

The two identities:

1. \[\tan^2(\theta) + 1 = \sec^{2}(\theta)\]
2. \[1 + \cot^2(\theta) = \text{cosec}^{2}(\theta)\]

** Addition Formula
*** Sin / Cos

\[\sin(A \pm B) = \sin(A)\cos(B) \pm \cos(A)\sin(B)\]

\[\cos(A \pm B) = \cos(A)\cos(B) \mp \sin(A)\sin(B)\]

*** Tan

The equivalent expression for $\tan(A \pm B)$ is derived by combining these examples:

- \[\tan(A \pm B) = \dfrac{\sin(A \pm B)}{\cos(A \mp B)}\]

- \[\tan(A \pm B) = \dfrac{\sin(A)\cos(B) \pm \cos(A)\sin(B)}{\cos(A)\cos(B) \mp \sin(A)\sin(B)}\]

- \[\tan(A \pm B) = \cfrac{\cfrac{\sin(A)\cos(B)}{\cos(A)\cos(B)} \pm \cfrac{\cos(A)\sin(B)}{\cos(A)\cos(B)}}{\cfrac{\cos(A)\cos(B)}{\cos(A)\cos(B)} \mp \cfrac{\sin(A)\sin(B)}{\cos(A)\cos(B)}}\]

The result is:

\[\tan(A \pm B) = \dfrac{\tan(A) \pm \tan(B)}{1 \mp \tan(A)\tan(B)}\]

*** Double Angles

Seeing as $2x = x + x$, there is a special case for the trigonometric addition formula.

\[ \begin{aligned} \sin(2x) = \sin(x + x) = \\ \sin(x)\cos(x) + \cos(x)\sin(x) = \\ 2\cos(x)\sin(x)  \text{ } \text{ } \text{ } \end{aligned}\]

\[\begin{aligned} \cos(2x) = \cos(x + x) = \\ \cos(x)\cos(x) - \sin(x)\sin(x) = \\ 1 - 2\sin^2(x) = \\ 2\cos^2(x) - 1   \text{ } \text{ } \text{ } \end{aligned} \]

* Differentiation
** Exponential and Logs
** Chain Rule
** Product Rule

\[ \dfrac{d}{{dx}}\left( {f\left( x \right) \boldsymbol{\cdot} g\left( x \right)} \right) = f\left( x \right)\boldsymbol{\cdot}\dfrac{d}{{dx}}g\left( x \right) + \dfrac{d}{{dx}}f\left( x \right)\boldsymbol{\cdot}g\left( x \right) \]

If $u$ and $v$ are functions of $x$, this expression can also be written:

\[y = uv  \text{ } \text{ } \text{ } \Rightarrow \text{ } \text{ } \text{ } \dfrac{dy}{dx} = u \dfrac{dv}{dx} + v \dfrac{du}{dx}\]

** Quotient Rule
** Parametrics
** Connected Rates of Change
